ok

SStructTT/SStruct/Runtime/Normalize.lean
@@ -17,3 +17,92 @@ theorem Resolved.normalize {H : Heap Srt} {a b c A} :
   have ⟨a', b', rs', _, st⟩ := rs.preservation st'
   apply ih <;> try assumption
   cases rs'; assumption
+
+def Measure : State Srt -> State Srt -> Prop  :=
+  InvImage (. < .) (fun m => measure m.2)
+
+lemma measure_decrease {H1 H2 : Heap Srt} {m1 m2} :
+    (Union Step0 Step1) (H1, m1) (H2, m2) -> measure m2 < measure m1 := by
+  intro st; induction m1 generalizing H1 H2 m2
+  all_goals simp_all
+  case var =>
+    cases st with
+    | inl st => cases st
+    | inr st => cases st
+  case lam =>
+    cases st with
+    | inl st => cases st
+    | inr st => cases st; simp
+  case app ihm ihn =>
+    cases st with
+    | inl st =>
+      cases st
+      case app_M st => simp[ihm (Or.inl st)]
+      case app_N st => simp[ihn (Or.inl st)]
+    | inr st =>
+      cases st
+      case app_M st => simp[ihm (Or.inr st)]
+      case app_N st => simp[ihn (Or.inr st)]
+  case tup ihm ihn =>
+    cases st with
+    | inl st =>
+      cases st
+      case tup_M st => simp[ihm (Or.inl st)]
+      case tup_N st => simp[ihn (Or.inl st)]
+    | inr st =>
+      cases st
+      case tup_M st => simp[ihm (Or.inr st)]
+      case tup_N st => simp[ihn (Or.inr st)]
+      case alloc_box => simp
+      case alloc_tup => simp
+  case prj ihm ihn =>
+    cases st with
+    | inl st =>
+      cases st
+      case prj_M st => simp[ihm (Or.inl st)]
+    | inr st =>
+      cases st
+      case prj_M st => simp[ihm (Or.inr st)]
+  case tt =>
+    cases st with
+    | inl st => cases st
+    | inr st => cases st; simp
+  case ff =>
+    cases st with
+    | inl st => cases st
+    | inr st => cases st; simp
+  case ite ihm ihn1 ihn2 =>
+    cases st with
+    | inl st =>
+      cases st
+      case ite_M st => simp[ihm (Or.inl st)]
+    | inr st =>
+      cases st
+      case ite_M st => simp[ihm (Or.inr st)]
+  case drop ihm ihn =>
+    cases st with
+    | inl st => cases st; simp
+    | inr st => cases st
+  case ptr =>
+    cases st with
+    | inl st => cases st
+    | inr st => cases st
+  case null =>
+    cases st with
+    | inl st => cases st
+    | inr st => cases st
+
+lemma measure_subrelation :
+    Subrelation (flip (@Union (State Srt) Step0 Step1)) Measure := by
+  intro ⟨H1, m1⟩ ⟨H2, m2⟩ st
+  apply measure_decrease st
+
+lemma wf_initial_steps : WellFounded (flip (@Union (State Srt) Step0 Step1)) := by
+  apply Subrelation.wf (@measure_subrelation Srt ord)
+  apply InvImage.wf
+  apply Nat.lt_wfRel.wf
+
+lemma sn_initial_steps {m : State Srt} : SN (Union Step0 Step1) m := by
+  have ⟨acc⟩ := @wf_initial_steps Srt ord
+  apply SN.ofAcc
+  apply acc
